word-ram/proofs/Lax13Proofs.lean
@@ -24,6 +24,8 @@ import Lax13Proofs.Refine.NREST.Pw
 import Lax13Proofs.Refine.NREST.Sanity
 import Lax13Proofs.Refine.NREST.Rec
 import Lax13Proofs.Refine.NREST.Combinators
+import Lax13Proofs.Refine.Autoref.Attrs
+import Lax13Proofs.Refine.Autoref.Relators
 import Lax13Proofs.Refine.NREST.DataRefinement
 import Lax13Proofs.Refine.NREST.TimeRefinement
 import Lax13Proofs.Refine.NREST.BackwardsReasoning
